convert-hs-to-coq/Decode_preamble.v
@@ -1,0 +1,3 @@
+Require Coq.ZArith.BinInt.
+Local Open Scope Z_scope.
+
