src/Decode.v
@@ -1,484 +1,898 @@
-Require Import Coq.omega.Omega.
-Require Import riscv.util.Decidable.
-Require Import riscv.util.NameWithEq.
-Require Import riscv.RiscvBitWidths.
-Require Import riscv.Utility.
-Require Import bbv.BinNotationZ.
-Require Import bbv.HexNotationZ.
+(* Default settings (from HsToCoq.Coq.Preamble) *)
 
+Generalizable All Variables.
+
+Unset Implicit Arguments.
+Set Maximal Implicit Insertion.
+Unset Strict Implicit.
+Unset Printing Implicit Defensive.
+
+Require Coq.Program.Tactics.
+Require Coq.Program.Wf.
+
+(* Preamble *)
+
+Require Coq.ZArith.BinInt.
 Local Open Scope Z_scope.
 
-Notation "a <|> b" := (Z.lor a b) (at level 50, left associativity).
-
-Section Instructions.
-
-Context {Name: NameWithEq}. (* register name *)
-Notation Register := (@name Name).
-
-Definition Imm := Z.
-
-Inductive Instruction : Set :=
-(* begin instructions *)
-  | InvalidInstruction
-
-  | Lb(rd: Register)(rs1: Register)(oimm12: MachineInt)
-  | Lh(rd: Register)(rs1: Register)(oimm12: MachineInt)
-  | Lw(rd: Register)(rs1: Register)(oimm12: MachineInt)
-  | Ld(rd: Register)(rs1: Register)(oimm12: MachineInt)
-  | Lbu(rd: Register)(rs1: Register)(oimm12: MachineInt)
-  | Lhu(rd: Register)(rs1: Register)(oimm12: MachineInt)
-  | Lwu(rd: Register)(rs1: Register)(oimm12: MachineInt)
-
-  | Fence(pred: MachineInt)(succ: MachineInt)
-  | Fence_i
-
-  | Addi(rd: Register)(rs1: Register)(imm12: MachineInt)
-  | Slli(rd: Register)(rs1: Register)(shamt6: MachineInt)
-  | Slti(rd: Register)(rs1: Register)(imm12: MachineInt)
-  | Sltiu(rd: Register)(rs1: Register)(imm12: MachineInt)
-  | Xori(rd: Register)(rs1: Register)(imm12: MachineInt)
-  | Ori(rd: Register)(rs1: Register)(imm12: MachineInt)
-  | Andi(rd: Register)(rs1: Register)(imm12: MachineInt)
-  | Srli(rd: Register)(rs1: Register)(shamt6: MachineInt)
-  | Srai(rd: Register)(rs1: Register)(shamt6: MachineInt)
-
-  | Auipc(rd: Register)(oimm20: MachineInt)
-
-  | Addiw(rd: Register)(rs1: Register)(imm12: MachineInt)
-  | Slliw(rd: Register)(rs1: Register)(shamt5: MachineInt)
-  | Srliw(rd: Register)(rs1: Register)(shamt5: MachineInt)
-  | Sraiw(rd: Register)(rs1: Register)(shamt5: MachineInt)
-
-  | Sb(rs1: Register)(rs2: Register)(simm12: MachineInt)
-  | Sh(rs1: Register)(rs2: Register)(simm12: MachineInt)
-  | Sw(rs1: Register)(rs2: Register)(simm12: MachineInt)
-  | Sd(rs1: Register)(rs2: Register)(simm12: MachineInt)
-
-  | Add(rd: Register)(rs1: Register)(rs2: Register)
-  | Sub(rd: Register)(rs1: Register)(rs2: Register)
-  | Sll(rd: Register)(rs1: Register)(rs2: Register)
-  | Slt(rd: Register)(rs1: Register)(rs2: Register)
-  | Sltu(rd: Register)(rs1: Register)(rs2: Register)
-  | Xor(rd: Register)(rs1: Register)(rs2: Register)
-  | Srl(rd: Register)(rs1: Register)(rs2: Register)
-  | Sra(rd: Register)(rs1: Register)(rs2: Register)
-  | Or(rd: Register)(rs1: Register)(rs2: Register)
-  | And(rd: Register)(rs1: Register)(rs2: Register)
-  | Mul(rd: Register)(rs1: Register)(rs2: Register)
-  | Mulh(rd: Register)(rs1: Register)(rs2: Register)
-  | Mulhsu(rd: Register)(rs1: Register)(rs2: Register)
-  | Mulhu(rd: Register)(rs1: Register)(rs2: Register)
-  | Div(rd: Register)(rs1: Register)(rs2: Register)
-  | Divu(rd: Register)(rs1: Register)(rs2: Register)
-  | Rem(rd: Register)(rs1: Register)(rs2: Register)
-  | Remu(rd: Register)(rs1: Register)(rs2: Register)
-
-  | Lui(rd: Register)(imm20: MachineInt)
-
-  | Addw(rd: Register)(rs1: Register)(rs2: Register)
-  | Subw(rd: Register)(rs1: Register)(rs2: Register)
-  | Sllw(rd: Register)(rs1: Register)(rs2: Register)
-  | Srlw(rd: Register)(rs1: Register)(rs2: Register)
-  | Sraw(rd: Register)(rs1: Register)(rs2: Register)
-  | Mulw(rd: Register)(rs1: Register)(rs2: Register)
-  | Divw(rd: Register)(rs1: Register)(rs2: Register)
-  | Divuw(rd: Register)(rs1: Register)(rs2: Register)
-  | Remw(rd: Register)(rs1: Register)(rs2: Register)
-  | Remuw(rd: Register)(rs1: Register)(rs2: Register)
-
-  | Beq(rs1: Register)(rs2: Register)(sbimm12: MachineInt)
-  | Bne(rs1: Register)(rs2: Register)(sbimm12: MachineInt)
-  | Blt(rs1: Register)(rs2: Register)(sbimm12: MachineInt)
-  | Bge(rs1: Register)(rs2: Register)(sbimm12: MachineInt)
-  | Bltu(rs1: Register)(rs2: Register)(sbimm12: MachineInt)
-  | Bgeu(rs1: Register)(rs2: Register)(sbimm12: MachineInt)
-
-  | Jalr(rd: Register)(rs1: Register)(oimm12: MachineInt)
-
-  | Jal(rd: Register)(jimm20: MachineInt)
-
-  | Ecall
-  | Ebreak
-  | Uret
-  | Sret
-  | Mret
-  | Wfi
-  | Sfence_vm(rs1: Register)(rs2: Register)
-
-  | Csrrw(rd: Register)(rs1: Register)(csr12: MachineInt)
-  | Csrrs(rd: Register)(rs1: Register)(csr12: MachineInt)
-  | Csrrc(rd: Register)(rs1: Register)(csr12: MachineInt)
-  | Csrrwi(rd: Register)(zimm: MachineInt)(csr12: MachineInt)
-  | Csrrsi(rd: Register)(zimm: MachineInt)(csr12: MachineInt)
-  | Csrrci(rd: Register)(zimm: MachineInt)(csr12: MachineInt)
-(* end instructions *)
-.
-
-End Instructions.
-
-(* Note: we could also use this notation:
-Eval cbv in (1~0~1~0)%positive.
-But it doesn't allow leading zeros, nor zero values. *)
-
-(* begin constants *)
-
-Definition opcode_LOAD       := Ob"0000011".
-Definition opcode_LOAD_FP    := Ob"0000111".
-Definition opcode_MISC_MEM   := Ob"0001111".
-Definition opcode_OP_IMM     := Ob"0010011".
-Definition opcode_AUIPC      := Ob"0010111".
-Definition opcode_OP_IMM_32  := Ob"0011011".
-
-Definition opcode_STORE      := Ob"0100011".
-Definition opcode_STORE_FP   := Ob"0100111".
-Definition opcode_AMO        := Ob"0101111".
-Definition opcode_OP         := Ob"0110011".
-Definition opcode_LUI        := Ob"0110111".
-Definition opcode_OP_32      := Ob"0111011".
-
-Definition opcode_MADD       := Ob"1000011".
-Definition opcode_MSUB       := Ob"1000111".
-Definition opcode_NMSUB      := Ob"1001011".
-Definition opcode_NMADD      := Ob"1001111".
-Definition opcode_OP_FP      := Ob"1010011".
-
-Definition opcode_BRANCH     := Ob"1100011".
-Definition opcode_JALR       := Ob"1100111".
-Definition opcode_JAL        := Ob"1101111".
-Definition opcode_SYSTEM     := Ob"1110011".
-
-(* LOAD sub-opcodes *)
-Definition funct3_LB   := Ob"000".
-Definition funct3_LH   := Ob"001".
-Definition funct3_LW   := Ob"010".
-Definition funct3_LD   := Ob"011".
-Definition funct3_LBU  := Ob"100".
-Definition funct3_LHU  := Ob"101".
-Definition funct3_LWU  := Ob"110".
-
-(* MISC_MEM sub-opcodes *)
-Definition funct3_FENCE    := Ob"000".
-Definition funct3_FENCE_I  := Ob"001".
-
-(* OP_IMM sub-opcodes *)
-Definition funct3_ADDI   := Ob"000".
-Definition funct3_SLLI   := Ob"001".
-Definition funct3_SLTI   := Ob"010".
-Definition funct3_SLTIU  := Ob"011".
-Definition funct3_XORI   := Ob"100".
-Definition funct3_SRLI   := Ob"101".
-Definition funct3_SRAI   := Ob"101".
-Definition funct3_ORI    := Ob"110".
-Definition funct3_ANDI   := Ob"111".
-
-(* OP_IMM.SLLI/SRLI/SRAI for RV32 *)
-Definition funct7_SLLI   := Ob"0000000".
-Definition funct7_SRLI   := Ob"0000000".
-Definition funct7_SRAI   := Ob"0100000".
-(* OP_IMM.SLLI/SRLI/SRAI for RV64 *)
-Definition funct6_SLLI   := Ob"000000".
-Definition funct6_SRLI   := Ob"000000".
-Definition funct6_SRAI   := Ob"010000".
 
-(* OP_IMM_32 sub-opcodes (RV64 only) *)
-Definition funct3_ADDIW  := Ob"000".
+(* Converted imports: *)
+
+Require Coq.Init.Datatypes.
+Require Import Coq.ZArith.BinInt.
+Require Import Utility.
+
+(* Converted type declarations: *)
+
+Definition Register :=
+  Z%type.
+
+Definition Opcode :=
+  Z%type.
+
+Inductive InstructionSet : Type
+  := RV32I : InstructionSet
+  |  RV32IM : InstructionSet
+  |  RV64I : InstructionSet
+  |  RV64IM : InstructionSet.
+
+Inductive InstructionM64 : Type
+  := Mulw : Register -> Register -> Register -> InstructionM64
+  |  Divw : Register -> Register -> Register -> InstructionM64
+  |  Divuw : Register -> Register -> Register -> InstructionM64
+  |  Remw : Register -> Register -> Register -> InstructionM64
+  |  Remuw : Register -> Register -> Register -> InstructionM64
+  |  InvalidM64 : InstructionM64.
+
+Inductive InstructionM : Type
+  := Mul : Register -> Register -> Register -> InstructionM
+  |  Mulh : Register -> Register -> Register -> InstructionM
+  |  Mulhsu : Register -> Register -> Register -> InstructionM
+  |  Mulhu : Register -> Register -> Register -> InstructionM
+  |  Div : Register -> Register -> Register -> InstructionM
+  |  Divu : Register -> Register -> Register -> InstructionM
+  |  Rem : Register -> Register -> Register -> InstructionM
+  |  Remu : Register -> Register -> Register -> InstructionM
+  |  InvalidM : InstructionM.
+
+Inductive InstructionI64 : Type
+  := Ld : Register -> Register -> Z -> InstructionI64
+  |  Lwu : Register -> Register -> Z -> InstructionI64
+  |  Addiw : Register -> Register -> Z -> InstructionI64
+  |  Slliw : Register -> Register -> Z -> InstructionI64
+  |  Srliw : Register -> Register -> Z -> InstructionI64
+  |  Sraiw : Register -> Register -> Z -> InstructionI64
+  |  Sd : Register -> Register -> Z -> InstructionI64
+  |  Addw : Register -> Register -> Register -> InstructionI64
+  |  Subw : Register -> Register -> Register -> InstructionI64
+  |  Sllw : Register -> Register -> Register -> InstructionI64
+  |  Srlw : Register -> Register -> Register -> InstructionI64
+  |  Sraw : Register -> Register -> Register -> InstructionI64
+  |  InvalidI64 : InstructionI64.
+
+Inductive InstructionI : Type
+  := Lb : Register -> Register -> Z -> InstructionI
+  |  Lh : Register -> Register -> Z -> InstructionI
+  |  Lw : Register -> Register -> Z -> InstructionI
+  |  Lbu : Register -> Register -> Z -> InstructionI
+  |  Lhu : Register -> Register -> Z -> InstructionI
+  |  Fence : Z -> Z -> InstructionI
+  |  Fence_i : InstructionI
+  |  Addi : Register -> Register -> Z -> InstructionI
+  |  Slli : Register -> Register -> Z -> InstructionI
+  |  Slti : Register -> Register -> Z -> InstructionI
+  |  Sltiu : Register -> Register -> Z -> InstructionI
+  |  Xori : Register -> Register -> Z -> InstructionI
+  |  Ori : Register -> Register -> Z -> InstructionI
+  |  Andi : Register -> Register -> Z -> InstructionI
+  |  Srli : Register -> Register -> Z -> InstructionI
+  |  Srai : Register -> Register -> Z -> InstructionI
+  |  Auipc : Register -> Z -> InstructionI
+  |  Sb : Register -> Register -> Z -> InstructionI
+  |  Sh : Register -> Register -> Z -> InstructionI
+  |  Sw : Register -> Register -> Z -> InstructionI
+  |  Add : Register -> Register -> Register -> InstructionI
+  |  Sub : Register -> Register -> Register -> InstructionI
+  |  Sll : Register -> Register -> Register -> InstructionI
+  |  Slt : Register -> Register -> Register -> InstructionI
+  |  Sltu : Register -> Register -> Register -> InstructionI
+  |  Xor : Register -> Register -> Register -> InstructionI
+  |  Srl : Register -> Register -> Register -> InstructionI
+  |  Sra : Register -> Register -> Register -> InstructionI
+  |  Or : Register -> Register -> Register -> InstructionI
+  |  And : Register -> Register -> Register -> InstructionI
+  |  Lui : Register -> Z -> InstructionI
+  |  Beq : Register -> Register -> Z -> InstructionI
+  |  Bne : Register -> Register -> Z -> InstructionI
+  |  Blt : Register -> Register -> Z -> InstructionI
+  |  Bge : Register -> Register -> Z -> InstructionI
+  |  Bltu : Register -> Register -> Z -> InstructionI
+  |  Bgeu : Register -> Register -> Z -> InstructionI
+  |  Jalr : Register -> Register -> Z -> InstructionI
+  |  Jal : Register -> Z -> InstructionI
+  |  InvalidI : InstructionI.
+
+Inductive InstructionCSR : Type
+  := Ecall : InstructionCSR
+  |  Ebreak : InstructionCSR
+  |  Uret : InstructionCSR
+  |  Sret : InstructionCSR
+  |  Mret : InstructionCSR
+  |  Wfi : InstructionCSR
+  |  Sfence_vm : Register -> Register -> InstructionCSR
+  |  Csrrw : Register -> Register -> Z -> InstructionCSR
+  |  Csrrs : Register -> Register -> Z -> InstructionCSR
+  |  Csrrc : Register -> Register -> Z -> InstructionCSR
+  |  Csrrwi : Register -> Z -> Z -> InstructionCSR
+  |  Csrrsi : Register -> Z -> Z -> InstructionCSR
+  |  Csrrci : Register -> Z -> Z -> InstructionCSR
+  |  InvalidCSR : InstructionCSR.
 
-Definition funct3_SLLIW  := Ob"001".
-Definition funct7_SLLIW  := Ob"0000000".
+Inductive Instruction : Type
+  := IInstruction : InstructionI -> Instruction
+  |  MInstruction : InstructionM -> Instruction
+  |  I64Instruction : InstructionI64 -> Instruction
+  |  M64Instruction : InstructionM64 -> Instruction
+  |  CSRInstruction : InstructionCSR -> Instruction
+  |  InvalidInstruction : Instruction.
+(* Converted value declarations: *)
 
-Definition funct3_SRLIW  := Ob"101".
-Definition funct7_SRLIW  := Ob"0000000".
+(* Translating `instance Show__Instruction' failed: OOPS! Cannot find
+   information for class Qualified "GHC.Show" "Show" unsupported *)
 
-Definition funct3_SRAIW  := Ob"101".
-Definition funct7_SRAIW  := Ob"0100000".
+(* Translating `instance Read__Instruction' failed: OOPS! Cannot find
+   information for class Qualified "GHC.Read" "Read" unsupported *)
 
-(* STORE sub-opcodes *)
-Definition funct3_SB  := Ob"000".
-Definition funct3_SH  := Ob"001".
-Definition funct3_SW  := Ob"010".
-Definition funct3_SD  := Ob"011".
-
-(* OP sub-opcodes *)
-Definition funct3_ADD   := Ob"000".
-Definition funct7_ADD   := Ob"0000000".
-
-Definition funct3_SUB   := Ob"000".
-Definition funct7_SUB   := Ob"0100000".
-
-Definition funct3_SLL   := Ob"001".
-Definition funct7_SLL   := Ob"0000000".
-
-Definition funct3_SLT   := Ob"010".
-Definition funct7_SLT   := Ob"0000000".
-
-Definition funct3_SLTU  := Ob"011".
-Definition funct7_SLTU  := Ob"0000000".
-
-Definition funct3_XOR   := Ob"100".
-Definition funct7_XOR   := Ob"0000000".
-
-Definition funct3_SRL   := Ob"101".
-Definition funct7_SRL   := Ob"0000000".
-
-Definition funct3_SRA   := Ob"101".
-Definition funct7_SRA   := Ob"0100000".
-
-Definition funct3_OR    := Ob"110".
-Definition funct7_OR    := Ob"0000000".
-
-Definition funct3_AND   := Ob"111".
-Definition funct7_AND   := Ob"0000000".
+(* Skipping instance Eq___Instruction *)
 
-(* OP sub-opcodes, M standard extension *)
-
-Definition funct3_MUL     := Ob"000".
-Definition funct7_MUL     := Ob"0000001".
-
-Definition funct3_MULH    := Ob"001".
-Definition funct7_MULH    := Ob"0000001".
-
-Definition funct3_MULHSU  := Ob"010".
-Definition funct7_MULHSU  := Ob"0000001".
-
-Definition funct3_MULHU   := Ob"011".
-Definition funct7_MULHU   := Ob"0000001".
-
-Definition funct3_DIV     := Ob"100".
-Definition funct7_DIV     := Ob"0000001".
-
-Definition funct3_DIVU    := Ob"101".
-Definition funct7_DIVU    := Ob"0000001".
-
-Definition funct3_REM     := Ob"110".
-Definition funct7_REM     := Ob"0000001".
-
-Definition funct3_REMU    := Ob"111".
-Definition funct7_REMU    := Ob"0000001".
-
-(* OP_32 sub-opcodes (RV64 only) *)
-Definition funct3_ADDW   := Ob"000".
-Definition funct7_ADDW   := Ob"0000000".
-
-Definition funct3_SUBW   := Ob"000".
-Definition funct7_SUBW   := Ob"0100000".
-
-Definition funct3_SLLW   := Ob"001".
-Definition funct7_SLLW   := Ob"0000000".
-
-Definition funct3_SRLW   := Ob"101".
-Definition funct7_SRLW   := Ob"0000000".
-
-Definition funct3_SRAW   := Ob"101".
-Definition funct7_SRAW   := Ob"0100000".
-
-(* OP_32 sub-opcodes, M standard extension (RV64 only) *)
-Definition funct3_MULW   := Ob"000".
-Definition funct7_MULW   := Ob"0000001".
-
-Definition funct3_DIVW   := Ob"100".
-Definition funct7_DIVW   := Ob"0000001".
-
-Definition funct3_DIVUW  := Ob"101".
-Definition funct7_DIVUW  := Ob"0000001".
-
-Definition funct3_REMW   := Ob"110".
-Definition funct7_REMW   := Ob"0000001".
-
-Definition funct3_REMUW  := Ob"111".
-Definition funct7_REMUW  := Ob"0000001".
-
-(* BRANCH sub-opcodes *)
-Definition funct3_BEQ   := Ob"000".
-Definition funct3_BNE   := Ob"001".
-Definition funct3_BLT   := Ob"100".
-Definition funct3_BGE   := Ob"101".
-Definition funct3_BLTU  := Ob"110".
-Definition funct3_BGEU  := Ob"111".
-
-(* SYSTEM sub-opcodes *)
-Definition funct3_PRIV    := Ob"000".
-(*- SYSTEM.PRIV sub-sub-opcodes *)
-Definition funct12_ECALL     := Ob"000000000000".
-Definition funct12_EBREAK    := Ob"000000000001".
-Definition funct12_URET      := Ob"000000000010".
-Definition funct12_SRET      := Ob"000100000010".
-Definition funct12_MRET      := Ob"001100000010".
-Definition funct12_WFI       := Ob"000100000101".
-
-Definition funct7_SFENCE_VM  := Ob"0001001".
-
-Definition funct3_CSRRW   := Ob"001".
-Definition funct3_CSRRS   := Ob"010".
-Definition funct3_CSRRC   := Ob"011".
-Definition funct3_CSRRWI  := Ob"101".
-Definition funct3_CSRRSI  := Ob"110".
-Definition funct3_CSRRCI  := Ob"111".
-
-(* TODO: sub-opcodes for LOAD_FP, STORE_FP, OP_FP *)
-(* TODO: sub-opcodes for AMO *)
-(* TODO: sub-opcodes for MADD, MSUB, NMSUB, NMADD *)
-
-(* end constants *)
-
-Definition shift := Z.shiftl.
-
-Local Instance ZName: NameWithEq := {|
-  name := Z
-|}.
-
-Local Open Scope bool_scope.
-
-Definition decode (xlen inst : MachineInt) : Instruction :=
-(* begin decode *)
-    let opcode  := bitSlice inst 0 7 in
-    let funct3  := bitSlice inst 12 15 in
-    let funct7  := bitSlice inst 25 32 in
-    let funct10 := (shift (bitSlice inst 25 32) 3) <|> (bitSlice inst 12 15) in
+(* Translating `instance Show__InstructionI' failed: OOPS! Cannot find
+   information for class Qualified "GHC.Show" "Show" unsupported *)
+
+(* Translating `instance Read__InstructionI' failed: OOPS! Cannot find
+   information for class Qualified "GHC.Read" "Read" unsupported *)
+
+(* Skipping instance Eq___InstructionI *)
+
+(* Translating `instance Show__InstructionM' failed: OOPS! Cannot find
+   information for class Qualified "GHC.Show" "Show" unsupported *)
+
+(* Translating `instance Read__InstructionM' failed: OOPS! Cannot find
+   information for class Qualified "GHC.Read" "Read" unsupported *)
+
+(* Skipping instance Eq___InstructionM *)
+
+(* Translating `instance Show__InstructionI64' failed: OOPS! Cannot find
+   information for class Qualified "GHC.Show" "Show" unsupported *)
+
+(* Translating `instance Read__InstructionI64' failed: OOPS! Cannot find
+   information for class Qualified "GHC.Read" "Read" unsupported *)
+
+(* Skipping instance Eq___InstructionI64 *)
+
+(* Translating `instance Show__InstructionM64' failed: OOPS! Cannot find
+   information for class Qualified "GHC.Show" "Show" unsupported *)
+
+(* Translating `instance Read__InstructionM64' failed: OOPS! Cannot find
+   information for class Qualified "GHC.Read" "Read" unsupported *)
+
+(* Skipping instance Eq___InstructionM64 *)
+
+(* Translating `instance Show__InstructionCSR' failed: OOPS! Cannot find
+   information for class Qualified "GHC.Show" "Show" unsupported *)
+
+(* Translating `instance Read__InstructionCSR' failed: OOPS! Cannot find
+   information for class Qualified "GHC.Read" "Read" unsupported *)
+
+(* Skipping instance Eq___InstructionCSR *)
+
+(* Translating `instance Show__InstructionSet' failed: OOPS! Cannot find
+   information for class Qualified "GHC.Show" "Show" unsupported *)
+
+(* Skipping instance Eq___InstructionSet *)
+
+Definition bitwidth : InstructionSet -> Z :=
+  fun arg_0__ =>
+    match arg_0__ with
+    | RV32I => 32
+    | RV32IM => 32
+    | RV64I => 64
+    | RV64IM => 64
+    end.
+
+Definition funct12_EBREAK : Z :=
+  1.
+
+Definition funct12_ECALL : Z :=
+  0.
+
+Definition funct12_MRET : Z :=
+  770.
+
+Definition funct12_SRET : Z :=
+  258.
+
+Definition funct12_URET : Z :=
+  2.
+
+Definition funct12_WFI : Z :=
+  261.
+
+Definition funct3_ADD : Z :=
+  0.
+
+Definition funct3_ADDI : Z :=
+  0.
+
+Definition funct3_ADDIW : Z :=
+  0.
+
+Definition funct3_ADDW : Z :=
+  0.
+
+Definition funct3_AND : Z :=
+  7.
+
+Definition funct3_ANDI : Z :=
+  7.
+
+Definition funct3_BEQ : Z :=
+  0.
+
+Definition funct3_BGE : Z :=
+  5.
+
+Definition funct3_BGEU : Z :=
+  7.
+
+Definition funct3_BLT : Z :=
+  4.
+
+Definition funct3_BLTU : Z :=
+  6.
+
+Definition funct3_BNE : Z :=
+  1.
+
+Definition funct3_CSRRC : Z :=
+  3.
+
+Definition funct3_CSRRCI : Z :=
+  7.
+
+Definition funct3_CSRRS : Z :=
+  2.
+
+Definition funct3_CSRRSI : Z :=
+  6.
+
+Definition funct3_CSRRW : Z :=
+  1.
+
+Definition funct3_CSRRWI : Z :=
+  5.
+
+Definition funct3_DIV : Z :=
+  4.
+
+Definition funct3_DIVU : Z :=
+  5.
+
+Definition funct3_DIVUW : Z :=
+  5.
+
+Definition funct3_DIVW : Z :=
+  4.
+
+Definition funct3_FENCE : Z :=
+  0.
+
+Definition funct3_FENCE_I : Z :=
+  1.
+
+Definition funct3_LB : Z :=
+  0.
+
+Definition funct3_LBU : Z :=
+  4.
+
+Definition funct3_LD : Z :=
+  3.
+
+Definition funct3_LH : Z :=
+  1.
+
+Definition funct3_LHU : Z :=
+  5.
+
+Definition funct3_LW : Z :=
+  2.
+
+Definition funct3_LWU : Z :=
+  6.
+
+Definition funct3_MUL : Z :=
+  0.
+
+Definition funct3_MULH : Z :=
+  1.
+
+Definition funct3_MULHSU : Z :=
+  2.
+
+Definition funct3_MULHU : Z :=
+  3.
+
+Definition funct3_MULW : Z :=
+  0.
+
+Definition funct3_OR : Z :=
+  6.
+
+Definition funct3_ORI : Z :=
+  6.
+
+Definition funct3_PRIV : Z :=
+  0.
+
+Definition funct3_REM : Z :=
+  6.
+
+Definition funct3_REMU : Z :=
+  7.
+
+Definition funct3_REMUW : Z :=
+  7.
+
+Definition funct3_REMW : Z :=
+  6.
+
+Definition funct3_SB : Z :=
+  0.
+
+Definition funct3_SD : Z :=
+  3.
+
+Definition funct3_SH : Z :=
+  1.
+
+Definition funct3_SLL : Z :=
+  1.
+
+Definition funct3_SLLI : Z :=
+  1.
+
+Definition funct3_SLLIW : Z :=
+  1.
+
+Definition funct3_SLLW : Z :=
+  1.
+
+Definition funct3_SLT : Z :=
+  2.
+
+Definition funct3_SLTI : Z :=
+  2.
+
+Definition funct3_SLTIU : Z :=
+  3.
+
+Definition funct3_SLTU : Z :=
+  3.
+
+Definition funct3_SRA : Z :=
+  5.
+
+Definition funct3_SRAI : Z :=
+  5.
+
+Definition funct3_SRAIW : Z :=
+  5.
+
+Definition funct3_SRAW : Z :=
+  5.
+
+Definition funct3_SRL : Z :=
+  5.
+
+Definition funct3_SRLI : Z :=
+  5.
+
+Definition funct3_SRLIW : Z :=
+  5.
+
+Definition funct3_SRLW : Z :=
+  5.
+
+Definition funct3_SUB : Z :=
+  0.
+
+Definition funct3_SUBW : Z :=
+  0.
+
+Definition funct3_SW : Z :=
+  2.
+
+Definition funct3_XOR : Z :=
+  4.
+
+Definition funct3_XORI : Z :=
+  4.
+
+Definition funct6_SLLI : Z :=
+  0.
+
+Definition funct6_SRAI : Z :=
+  16.
+
+Definition funct6_SRLI : Z :=
+  0.
+
+Definition funct7_ADD : Z :=
+  0.
+
+Definition funct7_ADDW : Z :=
+  0.
+
+Definition funct7_AND : Z :=
+  0.
+
+Definition funct7_DIV : Z :=
+  1.
+
+Definition funct7_DIVU : Z :=
+  1.
+
+Definition funct7_DIVUW : Z :=
+  1.
+
+Definition funct7_DIVW : Z :=
+  1.
+
+Definition funct7_MUL : Z :=
+  1.
+
+Definition funct7_MULH : Z :=
+  1.
+
+Definition funct7_MULHSU : Z :=
+  1.
+
+Definition funct7_MULHU : Z :=
+  1.
+
+Definition funct7_MULW : Z :=
+  1.
+
+Definition funct7_OR : Z :=
+  0.
+
+Definition funct7_REM : Z :=
+  1.
+
+Definition funct7_REMU : Z :=
+  1.
+
+Definition funct7_REMUW : Z :=
+  1.
+
+Definition funct7_REMW : Z :=
+  1.
+
+Definition funct7_SFENCE_VM : Z :=
+  9.
+
+Definition funct7_SLL : Z :=
+  0.
+
+Definition funct7_SLLIW : Z :=
+  0.
+
+Definition funct7_SLLW : Z :=
+  0.
+
+Definition funct7_SLT : Z :=
+  0.
+
+Definition funct7_SLTU : Z :=
+  0.
+
+Definition funct7_SRA : Z :=
+  32.
+
+Definition funct7_SRAIW : Z :=
+  32.
+
+Definition funct7_SRAW : Z :=
+  32.
+
+Definition funct7_SRL : Z :=
+  0.
+
+Definition funct7_SRLIW : Z :=
+  0.
+
+Definition funct7_SRLW : Z :=
+  0.
+
+Definition funct7_SUB : Z :=
+  32.
+
+Definition funct7_SUBW : Z :=
+  32.
+
+Definition funct7_XOR : Z :=
+  0.
+
+Definition opcode_AMO : Opcode :=
+  47.
+
+Definition opcode_AUIPC : Opcode :=
+  23.
+
+Definition opcode_BRANCH : Opcode :=
+  99.
+
+Definition opcode_JAL : Opcode :=
+  111.
+
+Definition opcode_JALR : Opcode :=
+  103.
+
+Definition opcode_LOAD : Opcode :=
+  3.
+
+Definition opcode_LOAD_FP : Opcode :=
+  7.
+
+Definition opcode_LUI : Opcode :=
+  55.
+
+Definition opcode_MADD : Opcode :=
+  67.
+
+Definition opcode_MISC_MEM : Opcode :=
+  15.
+
+Definition opcode_MSUB : Opcode :=
+  71.
+
+Definition opcode_NMADD : Opcode :=
+  79.
+
+Definition opcode_NMSUB : Opcode :=
+  75.
+
+Definition opcode_OP : Opcode :=
+  51.
+
+Definition opcode_OP_32 : Opcode :=
+  59.
+
+Definition opcode_OP_FP : Opcode :=
+  83.
+
+Definition opcode_OP_IMM : Opcode :=
+  19.
+
+Definition opcode_OP_IMM_32 : Opcode :=
+  27.
+
+Definition opcode_STORE : Opcode :=
+  35.
+
+Definition opcode_STORE_FP : Opcode :=
+  39.
+
+Definition opcode_SYSTEM : Opcode :=
+  115.
+
+Definition supportsM : InstructionSet -> bool :=
+  fun arg_0__ =>
+    match arg_0__ with
+    | RV32I => false
+    | RV32IM => true
+    | RV64I => false
+    | RV64IM => true
+    end.
+
+Definition decode : InstructionSet -> Z -> Instruction :=
+  fun iset inst =>
+    let zimm := bitSlice inst 15 20 in
+    let funct6 := bitSlice inst 26 32 in
+    let shamtHi := bitSlice inst 25 26 in
+    let shamtHiTest := orb (Z.eqb shamtHi 0) (Z.eqb (bitwidth iset) 64) in
+    let shamt6 := machineIntToShamt (bitSlice inst 20 26) in
+    let shamt5 := machineIntToShamt (bitSlice inst 20 25) in
+    let sbimm12 :=
+      signExtend 13 (Z.lor (Z.lor (Z.lor (Z.shiftl (bitSlice inst 31 32) 12) (Z.shiftl
+                                          (bitSlice inst 25 31) 5)) (Z.shiftl (bitSlice inst 8 12) 1)) (Z.shiftl
+                            (bitSlice inst 7 8) 11)) in
+    let simm12 :=
+      signExtend 12 (Z.lor (Z.shiftl (bitSlice inst 25 32) 5) (bitSlice inst 7 12)) in
+    let csr12 := bitSlice inst 20 32 in
+    let oimm12 := signExtend 12 (bitSlice inst 20 32) in
+    let imm12 := signExtend 12 (bitSlice inst 20 32) in
+    let jimm20 :=
+      signExtend 21 (Z.lor (Z.lor (Z.lor (Z.shiftl (bitSlice inst 31 32) 20) (Z.shiftl
+                                          (bitSlice inst 21 31) 1)) (Z.shiftl (bitSlice inst 20 21) 11)) (Z.shiftl
+                            (bitSlice inst 12 20) 12)) in
+    let oimm20 := signExtend 32 (Z.shiftl (bitSlice inst 12 32) 12) in
+    let imm20 := signExtend 32 (Z.shiftl (bitSlice inst 12 32) 12) in
+    let msb4 := bitSlice inst 28 32 in
+    let pred := bitSlice inst 24 28 in
+    let succ := bitSlice inst 20 24 in
+    let rs3 := bitSlice inst 27 32 in
+    let rs2 := bitSlice inst 20 25 in
+    let rs1 := bitSlice inst 15 20 in
+    let rd := bitSlice inst 7 12 in
     let funct12 := bitSlice inst 20 32 in
+    let funct10 := Z.lor (Z.shiftl (bitSlice inst 25 32) 3) (bitSlice inst 12 15) in
+    let funct7 := bitSlice inst 25 32 in
+    let funct3 := bitSlice inst 12 15 in
+    let opcode := bitSlice inst 0 7 in
+    let decodeI :=
+      if andb (Z.eqb opcode opcode_LOAD) (Z.eqb funct3 funct3_LB) : bool
+      then Lb rd rs1 oimm12 else
+      if andb (Z.eqb opcode opcode_LOAD) (Z.eqb funct3 funct3_LH) : bool
+      then Lh rd rs1 oimm12 else
+      if andb (Z.eqb opcode opcode_LOAD) (Z.eqb funct3 funct3_LW) : bool
+      then Lw rd rs1 oimm12 else
+      if andb (Z.eqb opcode opcode_LOAD) (Z.eqb funct3 funct3_LBU) : bool
+      then Lbu rd rs1 oimm12 else
+      if andb (Z.eqb opcode opcode_LOAD) (Z.eqb funct3 funct3_LHU) : bool
+      then Lhu rd rs1 oimm12 else
+      if andb (Z.eqb opcode opcode_MISC_MEM) (andb (Z.eqb rd 0) (andb (Z.eqb funct3
+                                                                             funct3_FENCE) (andb (Z.eqb rs1 0) (Z.eqb
+                                                                                                  msb4 0)))) : bool
+      then Fence pred succ else
+      if andb (Z.eqb opcode opcode_MISC_MEM) (andb (Z.eqb rd 0) (andb (Z.eqb funct3
+                                                                             funct3_FENCE_I) (andb (Z.eqb rs1 0) (Z.eqb
+                                                                                                    imm12 0)))) : bool
+      then Fence_i else
+      if andb (Z.eqb opcode opcode_OP_IMM) (Z.eqb funct3 funct3_ADDI) : bool
+      then Addi rd rs1 imm12 else
+      if andb (Z.eqb opcode opcode_OP_IMM) (Z.eqb funct3 funct3_SLTI) : bool
+      then Slti rd rs1 imm12 else
+      if andb (Z.eqb opcode opcode_OP_IMM) (Z.eqb funct3 funct3_SLTIU) : bool
+      then Sltiu rd rs1 imm12 else
+      if andb (Z.eqb opcode opcode_OP_IMM) (Z.eqb funct3 funct3_XORI) : bool
+      then Xori rd rs1 imm12 else
+      if andb (Z.eqb opcode opcode_OP_IMM) (Z.eqb funct3 funct3_ORI) : bool
+      then Ori rd rs1 imm12 else
+      if andb (Z.eqb opcode opcode_OP_IMM) (Z.eqb funct3 funct3_ANDI) : bool
+      then Andi rd rs1 imm12 else
+      if andb (Z.eqb opcode opcode_OP_IMM) (andb (Z.eqb funct3 funct3_SLLI) (andb
+                                                  (Z.eqb funct6 funct6_SLLI) shamtHiTest)) : bool
+      then Slli rd rs1 shamt6 else
+      if andb (Z.eqb opcode opcode_OP_IMM) (andb (Z.eqb funct3 funct3_SRLI) (andb
+                                                  (Z.eqb funct6 funct6_SRLI) shamtHiTest)) : bool
+      then Srli rd rs1 shamt6 else
+      if andb (Z.eqb opcode opcode_OP_IMM) (andb (Z.eqb funct3 funct3_SRAI) (andb
+                                                  (Z.eqb funct6 funct6_SRAI) shamtHiTest)) : bool
+      then Srai rd rs1 shamt6 else
+      if Z.eqb opcode opcode_AUIPC : bool then Auipc rd oimm20 else
+      if andb (Z.eqb opcode opcode_STORE) (Z.eqb funct3 funct3_SB) : bool
+      then Sb rs1 rs2 simm12 else
+      if andb (Z.eqb opcode opcode_STORE) (Z.eqb funct3 funct3_SH) : bool
+      then Sh rs1 rs2 simm12 else
+      if andb (Z.eqb opcode opcode_STORE) (Z.eqb funct3 funct3_SW) : bool
+      then Sw rs1 rs2 simm12 else
+      if andb (Z.eqb opcode opcode_OP) (andb (Z.eqb funct3 funct3_ADD) (Z.eqb funct7
+                                                                              funct7_ADD)) : bool
+      then Add rd rs1 rs2 else
+      if andb (Z.eqb opcode opcode_OP) (andb (Z.eqb funct3 funct3_SUB) (Z.eqb funct7
+                                                                              funct7_SUB)) : bool
+      then Sub rd rs1 rs2 else
+      if andb (Z.eqb opcode opcode_OP) (andb (Z.eqb funct3 funct3_SLL) (Z.eqb funct7
+                                                                              funct7_SLL)) : bool
+      then Sll rd rs1 rs2 else
+      if andb (Z.eqb opcode opcode_OP) (andb (Z.eqb funct3 funct3_SLT) (Z.eqb funct7
+                                                                              funct7_SLT)) : bool
+      then Slt rd rs1 rs2 else
+      if andb (Z.eqb opcode opcode_OP) (andb (Z.eqb funct3 funct3_SLTU) (Z.eqb funct7
+                                                                               funct7_SLTU)) : bool
+      then Sltu rd rs1 rs2 else
+      if andb (Z.eqb opcode opcode_OP) (andb (Z.eqb funct3 funct3_XOR) (Z.eqb funct7
+                                                                              funct7_XOR)) : bool
+      then Xor rd rs1 rs2 else
+      if andb (Z.eqb opcode opcode_OP) (andb (Z.eqb funct3 funct3_SRL) (Z.eqb funct7
+                                                                              funct7_SRL)) : bool
+      then Srl rd rs1 rs2 else
+      if andb (Z.eqb opcode opcode_OP) (andb (Z.eqb funct3 funct3_SRA) (Z.eqb funct7
+                                                                              funct7_SRA)) : bool
+      then Sra rd rs1 rs2 else
+      if andb (Z.eqb opcode opcode_OP) (andb (Z.eqb funct3 funct3_OR) (Z.eqb funct7
+                                                                             funct7_OR)) : bool
+      then Or rd rs1 rs2 else
+      if andb (Z.eqb opcode opcode_OP) (andb (Z.eqb funct3 funct3_AND) (Z.eqb funct7
+                                                                              funct7_AND)) : bool
+      then And rd rs1 rs2 else
+      if Z.eqb opcode opcode_LUI : bool then Lui rd imm20 else
+      if andb (Z.eqb opcode opcode_BRANCH) (Z.eqb funct3 funct3_BEQ) : bool
+      then Beq rs1 rs2 sbimm12 else
+      if andb (Z.eqb opcode opcode_BRANCH) (Z.eqb funct3 funct3_BNE) : bool
+      then Bne rs1 rs2 sbimm12 else
+      if andb (Z.eqb opcode opcode_BRANCH) (Z.eqb funct3 funct3_BLT) : bool
+      then Blt rs1 rs2 sbimm12 else
+      if andb (Z.eqb opcode opcode_BRANCH) (Z.eqb funct3 funct3_BGE) : bool
+      then Bge rs1 rs2 sbimm12 else
+      if andb (Z.eqb opcode opcode_BRANCH) (Z.eqb funct3 funct3_BLTU) : bool
+      then Bltu rs1 rs2 sbimm12 else
+      if andb (Z.eqb opcode opcode_BRANCH) (Z.eqb funct3 funct3_BGEU) : bool
+      then Bgeu rs1 rs2 sbimm12 else
+      if Z.eqb opcode opcode_JALR : bool then Jalr rd rs1 oimm12 else
+      if Z.eqb opcode opcode_JAL : bool then Jal rd jimm20 else
+      InvalidI in
+    let decodeM :=
+      if andb (Z.eqb opcode opcode_OP) (andb (Z.eqb funct3 funct3_MUL) (Z.eqb funct7
+                                                                              funct7_MUL)) : bool
+      then Mul rd rs1 rs2 else
+      if andb (Z.eqb opcode opcode_OP) (andb (Z.eqb funct3 funct3_MULH) (Z.eqb funct7
+                                                                               funct7_MULH)) : bool
+      then Mulh rd rs1 rs2 else
+      if andb (Z.eqb opcode opcode_OP) (andb (Z.eqb funct3 funct3_MULHSU) (Z.eqb
+                                              funct7 funct7_MULHSU)) : bool
+      then Mulhsu rd rs1 rs2 else
+      if andb (Z.eqb opcode opcode_OP) (andb (Z.eqb funct3 funct3_MULHU) (Z.eqb funct7
+                                                                                funct7_MULHU)) : bool
+      then Mulhu rd rs1 rs2 else
+      if andb (Z.eqb opcode opcode_OP) (andb (Z.eqb funct3 funct3_DIV) (Z.eqb funct7
+                                                                              funct7_DIV)) : bool
+      then Div rd rs1 rs2 else
+      if andb (Z.eqb opcode opcode_OP) (andb (Z.eqb funct3 funct3_DIVU) (Z.eqb funct7
+                                                                               funct7_DIVU)) : bool
+      then Divu rd rs1 rs2 else
+      if andb (Z.eqb opcode opcode_OP) (andb (Z.eqb funct3 funct3_REM) (Z.eqb funct7
+                                                                              funct7_REM)) : bool
+      then Rem rd rs1 rs2 else
+      if andb (Z.eqb opcode opcode_OP) (andb (Z.eqb funct3 funct3_REMU) (Z.eqb funct7
+                                                                               funct7_REMU)) : bool
+      then Remu rd rs1 rs2 else
+      InvalidM in
+    let decodeI64 :=
+      if andb (Z.eqb opcode opcode_LOAD) (Z.eqb funct3 funct3_LD) : bool
+      then Ld rd rs1 oimm12 else
+      if andb (Z.eqb opcode opcode_LOAD) (Z.eqb funct3 funct3_LWU) : bool
+      then Lwu rd rs1 oimm12 else
+      if andb (Z.eqb opcode opcode_OP_IMM_32) (Z.eqb funct3 funct3_ADDIW) : bool
+      then Addiw rd rs1 imm12 else
+      if andb (Z.eqb opcode opcode_OP_IMM_32) (andb (Z.eqb funct3 funct3_SLLIW) (Z.eqb
+                                                     funct7 funct7_SLLIW)) : bool
+      then Slliw rd rs1 shamt5 else
+      if andb (Z.eqb opcode opcode_OP_IMM_32) (andb (Z.eqb funct3 funct3_SRLIW) (Z.eqb
+                                                     funct7 funct7_SRLIW)) : bool
+      then Srliw rd rs1 shamt5 else
+      if andb (Z.eqb opcode opcode_OP_IMM_32) (andb (Z.eqb funct3 funct3_SRAIW) (Z.eqb
+                                                     funct7 funct7_SRAIW)) : bool
+      then Sraiw rd rs1 shamt5 else
+      if andb (Z.eqb opcode opcode_STORE) (Z.eqb funct3 funct3_SD) : bool
+      then Sd rs1 rs2 simm12 else
+      if andb (Z.eqb opcode opcode_OP_32) (andb (Z.eqb funct3 funct3_ADDW) (Z.eqb
+                                                 funct7 funct7_ADDW)) : bool
+      then Addw rd rs1 rs2 else
+      if andb (Z.eqb opcode opcode_OP_32) (andb (Z.eqb funct3 funct3_SUBW) (Z.eqb
+                                                 funct7 funct7_SUBW)) : bool
+      then Subw rd rs1 rs2 else
+      if andb (Z.eqb opcode opcode_OP_32) (andb (Z.eqb funct3 funct3_SLLW) (Z.eqb
+                                                 funct7 funct7_SLLW)) : bool
+      then Sllw rd rs1 rs2 else
+      if andb (Z.eqb opcode opcode_OP_32) (andb (Z.eqb funct3 funct3_SRLW) (Z.eqb
+                                                 funct7 funct7_SRLW)) : bool
+      then Srlw rd rs1 rs2 else
+      if andb (Z.eqb opcode opcode_OP_32) (andb (Z.eqb funct3 funct3_SRAW) (Z.eqb
+                                                 funct7 funct7_SRAW)) : bool
+      then Sraw rd rs1 rs2 else
+      InvalidI64 in
+    let decodeM64 :=
+      if andb (Z.eqb opcode opcode_OP_32) (andb (Z.eqb funct3 funct3_MULW) (Z.eqb
+                                                 funct7 funct7_MULW)) : bool
+      then Mulw rd rs1 rs2 else
+      if andb (Z.eqb opcode opcode_OP_32) (andb (Z.eqb funct3 funct3_DIVW) (Z.eqb
+                                                 funct7 funct7_DIVW)) : bool
+      then Divw rd rs1 rs2 else
+      if andb (Z.eqb opcode opcode_OP_32) (andb (Z.eqb funct3 funct3_DIVUW) (Z.eqb
+                                                 funct7 funct7_DIVUW)) : bool
+      then Divuw rd rs1 rs2 else
+      if andb (Z.eqb opcode opcode_OP_32) (andb (Z.eqb funct3 funct3_REMW) (Z.eqb
+                                                 funct7 funct7_REMW)) : bool
+      then Remw rd rs1 rs2 else
+      if andb (Z.eqb opcode opcode_OP_32) (andb (Z.eqb funct3 funct3_REMUW) (Z.eqb
+                                                 funct7 funct7_REMUW)) : bool
+      then Remuw rd rs1 rs2 else
+      InvalidM64 in
+    let decodeCSR :=
+      if andb (Z.eqb opcode opcode_SYSTEM) (andb (Z.eqb rd 0) (andb (Z.eqb funct3
+                                                                           funct3_PRIV) (andb (Z.eqb rs1 0) (Z.eqb
+                                                                                               funct12
+                                                                                               funct12_ECALL)))) : bool
+      then Ecall else
+      if andb (Z.eqb opcode opcode_SYSTEM) (andb (Z.eqb rd 0) (andb (Z.eqb funct3
+                                                                           funct3_PRIV) (andb (Z.eqb rs1 0) (Z.eqb
+                                                                                               funct12
+                                                                                               funct12_EBREAK)))) : bool
+      then Ebreak else
+      if andb (Z.eqb opcode opcode_SYSTEM) (andb (Z.eqb rd 0) (andb (Z.eqb funct3
+                                                                           funct3_PRIV) (andb (Z.eqb rs1 0) (Z.eqb
+                                                                                               funct12
+                                                                                               funct12_URET)))) : bool
+      then Uret else
+      if andb (Z.eqb opcode opcode_SYSTEM) (andb (Z.eqb rd 0) (andb (Z.eqb funct3
+                                                                           funct3_PRIV) (andb (Z.eqb rs1 0) (Z.eqb
+                                                                                               funct12
+                                                                                               funct12_SRET)))) : bool
+      then Sret else
+      if andb (Z.eqb opcode opcode_SYSTEM) (andb (Z.eqb rd 0) (andb (Z.eqb funct3
+                                                                           funct3_PRIV) (andb (Z.eqb rs1 0) (Z.eqb
+                                                                                               funct12
+                                                                                               funct12_MRET)))) : bool
+      then Mret else
+      if andb (Z.eqb opcode opcode_SYSTEM) (andb (Z.eqb rd 0) (andb (Z.eqb funct3
+                                                                           funct3_PRIV) (andb (Z.eqb rs1 0) (Z.eqb
+                                                                                               funct12
+                                                                                               funct12_WFI)))) : bool
+      then Wfi else
+      if andb (Z.eqb opcode opcode_SYSTEM) (Z.eqb funct3 funct3_CSRRW) : bool
+      then Csrrw rd rs1 csr12 else
+      if andb (Z.eqb opcode opcode_SYSTEM) (Z.eqb funct3 funct3_CSRRS) : bool
+      then Csrrs rd rs1 csr12 else
+      if andb (Z.eqb opcode opcode_SYSTEM) (Z.eqb funct3 funct3_CSRRC) : bool
+      then Csrrc rd rs1 csr12 else
+      if andb (Z.eqb opcode opcode_SYSTEM) (Z.eqb funct3 funct3_CSRRWI) : bool
+      then Csrrwi rd zimm csr12 else
+      if andb (Z.eqb opcode opcode_SYSTEM) (Z.eqb funct3 funct3_CSRRSI) : bool
+      then Csrrsi rd zimm csr12 else
+      if andb (Z.eqb opcode opcode_SYSTEM) (Z.eqb funct3 funct3_CSRRCI) : bool
+      then Csrrci rd zimm csr12 else
+      InvalidCSR in
+    let resultCSR :=
+      match decodeCSR with
+      | InvalidCSR => nil
+      | _ => cons (CSRInstruction decodeCSR) nil
+      end in
+    let resultM64 :=
+      match decodeM64 with
+      | InvalidM64 => nil
+      | _ => cons (M64Instruction decodeM64) nil
+      end in
+    let resultI64 :=
+      match decodeI64 with
+      | InvalidI64 => nil
+      | _ => cons (I64Instruction decodeI64) nil
+      end in
+    let resultM :=
+      match decodeM with
+      | InvalidM => nil
+      | _ => cons (MInstruction decodeM) nil
+      end in
+    let resultI :=
+      match decodeI with
+      | InvalidI => nil
+      | _ => cons (IInstruction decodeI) nil
+      end in
+    let results : list Instruction :=
+      Coq.Init.Datatypes.app resultI (Coq.Init.Datatypes.app (if supportsM iset : bool
+                                                              then resultM
+                                                              else nil) (Coq.Init.Datatypes.app (if Z.eqb (bitwidth
+                                                                                                           iset)
+                                                                                                          64 : bool
+                                                                                                 then resultI64
+                                                                                                 else nil)
+                                                                                                (Coq.Init.Datatypes.app
+                                                                                                 (if andb (Z.eqb
+                                                                                                           (bitwidth
+                                                                                                            iset) 64)
+                                                                                                          (supportsM
+                                                                                                           iset) : bool
+                                                                                                  then resultM64
+                                                                                                  else nil)
+                                                                                                 resultCSR))) in
+    match results with
+    | cons singleResult nil => singleResult
+    | nil => InvalidInstruction
+    | _ => InvalidInstruction
+    end.
 
-    let rd      := bitSlice inst 7 12 in
-    let rs1     := bitSlice inst 15 20 in
-    let rs2     := bitSlice inst 20 25 in
-    let rs3     := bitSlice inst 27 32 in
-
-    let succ    := bitSlice inst 20 24 in
-    let pred    := bitSlice inst 24 28 in
-    let msb4    := bitSlice inst 28 32 in
-
-    let imm20   := signExtend 32 (shift (bitSlice inst 12 32) 12) in
-    let oimm20  := signExtend 32 (shift (bitSlice inst 12 32) 12) in
-
-    let jimm20  := signExtend 21 ((shift (bitSlice inst 31 32) 20  <|>
-                                shift (bitSlice inst 21 31) 1  <|>
-                                shift (bitSlice inst 20 21) 11 <|>
-                                shift (bitSlice inst 12 20) 12)) in
-
-    let imm12   := signExtend 12 (bitSlice inst 20 32) in
-    let oimm12  := signExtend 12 (bitSlice inst 20 32) in
-
-    let csr12   := bitSlice inst 20 32 in
-
-    let simm12  := signExtend 12 (shift (bitSlice inst 25 32) 5 <|> bitSlice inst 7 12) in
-
-    let sbimm12 := signExtend 13 ((shift (bitSlice inst 31 32) 12 <|>
-                                shift (bitSlice inst 25 31) 5 <|>
-                                shift (bitSlice inst 8 12) 1  <|>
-                                shift (bitSlice inst 7 8) 11)) in
-
-    let shamt5  := bitSlice inst 20 25 in
-    let shamt6  := bitSlice inst 20 26 in
-    let funct6  := bitSlice inst 26 32 in
-
-    let zimm    := bitSlice inst 15 20 in
-
-    if (opcode =? opcode_LOAD) && (funct3 =? funct3_LB) then Lb rd rs1 oimm12 else
-    if (opcode =? opcode_LOAD) && (funct3 =? funct3_LH) then Lh rd rs1 oimm12 else
-    if (opcode =? opcode_LOAD) && (funct3 =? funct3_LW) then Lw rd rs1 oimm12 else
-    if (opcode =? opcode_LOAD) && (funct3 =? funct3_LBU) then Lbu rd rs1 oimm12 else
-    if (opcode =? opcode_LOAD) && (funct3 =? funct3_LHU) then Lhu rd rs1 oimm12 else
-
-    if (opcode =? opcode_MISC_MEM) && (rd =? 0) && (funct3 =? funct3_FENCE) && (rs1 =? 0) && (msb4 =? 0) then Fence pred succ else
-    if (opcode =? opcode_MISC_MEM) && (rd =? 0) && (funct3 =? funct3_FENCE_I) && (rs1 =? 0) && (imm12 =? 0) then Fence_i  else
-
-    if (opcode =? opcode_OP_IMM) && (funct3 =? funct3_ADDI) then Addi rd rs1 imm12 else
-    if (opcode =? opcode_OP_IMM) && (funct3 =? funct3_SLLI) && (funct7 =? funct7_SLLI) && (xlen =? 32) then Slli rd rs1 shamt5 else
-    if (opcode =? opcode_OP_IMM) && (funct3 =? funct3_SLTI) then Slti rd rs1 imm12 else
-    if (opcode =? opcode_OP_IMM) && (funct3 =? funct3_SLTIU) then Sltiu rd rs1 imm12 else
-    if (opcode =? opcode_OP_IMM) && (funct3 =? funct3_XORI) then Xori rd rs1 imm12 else
-    if (opcode =? opcode_OP_IMM) && (funct3 =? funct3_ORI) then Ori rd rs1 imm12 else
-    if (opcode =? opcode_OP_IMM) && (funct3 =? funct3_ANDI) then Andi rd rs1 imm12 else
-    if (opcode =? opcode_OP_IMM) && (funct3 =? funct3_SRLI) && (funct7 =? funct7_SRLI) && (xlen =? 32) then Srli rd rs1 shamt5 else
-    if (opcode =? opcode_OP_IMM) && (funct3 =? funct3_SRAI) && (funct7 =? funct7_SRAI) && (xlen =? 32) then Srai rd rs1 shamt5 else
-
-    if (opcode =? opcode_AUIPC) then Auipc rd oimm20 else
-
-    if (opcode =? opcode_STORE) && (funct3 =? funct3_SB) then Sb rs1 rs2 simm12 else
-    if (opcode =? opcode_STORE) && (funct3 =? funct3_SH) then Sh rs1 rs2 simm12 else
-    if (opcode =? opcode_STORE) && (funct3 =? funct3_SW) then Sw rs1 rs2 simm12 else
-
-    if (opcode =? opcode_OP) && (funct3 =? funct3_ADD) && (funct7 =? funct7_ADD) then Add rd rs1 rs2 else
-    if (opcode =? opcode_OP) && (funct3 =? funct3_SUB) && (funct7 =? funct7_SUB) then Sub rd rs1 rs2 else
-    if (opcode =? opcode_OP) && (funct3 =? funct3_SLL) && (funct7 =? funct7_SLL) then Sll rd rs1 rs2 else
-    if (opcode =? opcode_OP) && (funct3 =? funct3_SLT) && (funct7 =? funct7_SLT) then Slt rd rs1 rs2 else
-    if (opcode =? opcode_OP) && (funct3 =? funct3_SLTU) && (funct7 =? funct7_SLTU) then Sltu rd rs1 rs2 else
-    if (opcode =? opcode_OP) && (funct3 =? funct3_XOR) && (funct7 =? funct7_XOR) then Xor rd rs1 rs2 else
-    if (opcode =? opcode_OP) && (funct3 =? funct3_SRL) && (funct7 =? funct7_SRL) then Srl rd rs1 rs2 else
-    if (opcode =? opcode_OP) && (funct3 =? funct3_SRA) && (funct7 =? funct7_SRA) then Sra rd rs1 rs2 else
-    if (opcode =? opcode_OP) && (funct3 =? funct3_OR) && (funct7 =? funct7_OR) then Or rd rs1 rs2 else
-    if (opcode =? opcode_OP) && (funct3 =? funct3_AND) && (funct7 =? funct7_AND) then And rd rs1 rs2 else
-
-    if (opcode =? opcode_OP) && (funct3 =? funct3_MUL) && (funct7 =? funct7_MUL) then Mul rd rs1 rs2 else
-    if (opcode =? opcode_OP) && (funct3 =? funct3_MULH) && (funct7 =? funct7_MULH) then Mulh rd rs1 rs2 else
-    if (opcode =? opcode_OP) && (funct3 =? funct3_MULHSU) && (funct7 =? funct7_MULHSU) then Mulhsu rd rs1 rs2 else
-    if (opcode =? opcode_OP) && (funct3 =? funct3_MULHU) && (funct7 =? funct7_MULHU) then Mulhu rd rs1 rs2 else
-    if (opcode =? opcode_OP) && (funct3 =? funct3_DIV) && (funct7 =? funct7_DIV) then Div rd rs1 rs2 else
-    if (opcode =? opcode_OP) && (funct3 =? funct3_DIVU) && (funct7 =? funct7_DIVU) then Divu rd rs1 rs2 else
-    if (opcode =? opcode_OP) && (funct3 =? funct3_REM) && (funct7 =? funct7_REM) then Rem rd rs1 rs2 else
-    if (opcode =? opcode_OP) && (funct3 =? funct3_REMU) && (funct7 =? funct7_REMU) then Remu rd rs1 rs2 else
-
-    if (opcode =? opcode_LUI) then Lui rd imm20 else
-
-    if (opcode =? opcode_BRANCH) && (funct3 =? funct3_BEQ) then Beq rs1 rs2 sbimm12 else
-    if (opcode =? opcode_BRANCH) && (funct3 =? funct3_BNE) then Bne rs1 rs2 sbimm12 else
-    if (opcode =? opcode_BRANCH) && (funct3 =? funct3_BLT) then Blt rs1 rs2 sbimm12 else
-    if (opcode =? opcode_BRANCH) && (funct3 =? funct3_BGE) then Bge rs1 rs2 sbimm12 else
-    if (opcode =? opcode_BRANCH) && (funct3 =? funct3_BLTU) then Bltu rs1 rs2 sbimm12 else
-    if (opcode =? opcode_BRANCH) && (funct3 =? funct3_BGEU) then Bgeu rs1 rs2 sbimm12 else
-
-    if (opcode =? opcode_JALR) then Jalr rd rs1 oimm12 else
-
-    if (opcode =? opcode_JAL) then Jal rd jimm20 else
-
-    if (opcode =? opcode_SYSTEM) && (rd =? 0) && (funct3 =? funct3_PRIV) && (rs1 =? 0) && (funct12 =? funct12_ECALL) then Ecall  else
-    if (opcode =? opcode_SYSTEM) && (rd =? 0) && (funct3 =? funct3_PRIV) && (rs1 =? 0) && (funct12 =? funct12_EBREAK) then Ebreak  else
-    if (opcode =? opcode_SYSTEM) && (rd =? 0) && (funct3 =? funct3_PRIV) && (rs1 =? 0) && (funct12 =? funct12_URET) then Uret  else
-    if (opcode =? opcode_SYSTEM) && (rd =? 0) && (funct3 =? funct3_PRIV) && (rs1 =? 0) && (funct12 =? funct12_SRET) then Sret  else
-    if (opcode =? opcode_SYSTEM) && (rd =? 0) && (funct3 =? funct3_PRIV) && (rs1 =? 0) && (funct12 =? funct12_MRET) then Mret  else
-    if (opcode =? opcode_SYSTEM) && (rd =? 0) && (funct3 =? funct3_PRIV) && (rs1 =? 0) && (funct12 =? funct12_WFI) then Wfi  else
-
-    if (opcode =? opcode_SYSTEM) && (rd =? 0) && (funct3 =? funct3_PRIV) && (funct7 =? funct7_SFENCE_VM) then Sfence_vm rs1 rs2 else
-
-    if (opcode =? opcode_SYSTEM) && (funct3 =? funct3_CSRRW) then Csrrw rd rs1   csr12 else
-    if (opcode =? opcode_SYSTEM) && (funct3 =? funct3_CSRRS) then Csrrw rd rs1   csr12 else
-    if (opcode =? opcode_SYSTEM) && (funct3 =? funct3_CSRRC) then Csrrw rd rs1   csr12 else
-    if (opcode =? opcode_SYSTEM) && (funct3 =? funct3_CSRRWI) then Csrrwi rd zimm csr12 else
-    if (opcode =? opcode_SYSTEM) && (funct3 =? funct3_CSRRSI) then Csrrwi rd zimm csr12 else
-    if (opcode =? opcode_SYSTEM) && (funct3 =? funct3_CSRRCI) then Csrrwi rd zimm csr12 else
-
-    if (opcode =? opcode_LOAD) && (funct3 =? funct3_LD) && (xlen =? 64) then Ld rd rs1 oimm12 else
-    if (opcode =? opcode_LOAD) && (funct3 =? funct3_LWU) && (xlen =? 64) then Lwu rd rs1 oimm12 else
-
-    if (opcode =? opcode_OP_IMM) && (funct3 =? funct3_SLLI) && (funct6 =? funct6_SLLI) && (xlen =? 64) then Slli rd rs1 shamt6 else
-    if (opcode =? opcode_OP_IMM) && (funct3 =? funct3_SRLI) && (funct6 =? funct6_SRLI) && (xlen =? 64) then Srli rd rs1 shamt6 else
-    if (opcode =? opcode_OP_IMM) && (funct3 =? funct3_SRAI) && (funct6 =? funct6_SRAI) && (xlen =? 64) then Srai rd rs1 shamt6 else
-
-    if (opcode =? opcode_OP_IMM_32) && (funct3 =? funct3_ADDIW) && (xlen =? 64) then Addiw rd rs1 imm12 else
-    if (opcode =? opcode_OP_IMM_32) && (funct3 =? funct3_SLLIW) && (funct7 =? funct7_SLLIW) && (xlen =? 64) then Slliw rd rs1 shamt5 else
-    if (opcode =? opcode_OP_IMM_32) && (funct3 =? funct3_SRLIW) && (funct7 =? funct7_SRLIW) && (xlen =? 64) then Srliw rd rs1 shamt5 else
-    if (opcode =? opcode_OP_IMM_32) && (funct3 =? funct3_SRAIW) && (funct7 =? funct7_SRAIW) && (xlen =? 64) then Sraiw rd rs1 shamt5 else
-
-    if (opcode =? opcode_STORE) && (funct3 =? funct3_SD) && (xlen =? 64) then Sd rs1 rs2 simm12 else
-
-    if (opcode =? opcode_OP_32) && (funct3 =? funct3_ADDW) && (funct7 =? funct7_ADDW) && (xlen =? 64) then Addw rd rs1 rs2 else
-    if (opcode =? opcode_OP_32) && (funct3 =? funct3_SUBW) && (funct7 =? funct7_SUBW) && (xlen =? 64) then Subw rd rs1 rs2 else
-    if (opcode =? opcode_OP_32) && (funct3 =? funct3_SLLW) && (funct7 =? funct7_SLLW) && (xlen =? 64) then Sllw rd rs1 rs2 else
-    if (opcode =? opcode_OP_32) && (funct3 =? funct3_SRLW) && (funct7 =? funct7_SRLW) && (xlen =? 64) then Srlw rd rs1 rs2 else
-    if (opcode =? opcode_OP_32) && (funct3 =? funct3_SRAW) && (funct7 =? funct7_SRAW) && (xlen =? 64) then Sraw rd rs1 rs2 else
-
-    if (opcode =? opcode_OP_32) && (funct3 =? funct3_MULW) && (funct7 =? funct7_MULW) && (xlen =? 64) then Mulw rd rs1 rs2 else
-    if (opcode =? opcode_OP_32) && (funct3 =? funct3_DIVW) && (funct7 =? funct7_DIVW) && (xlen =? 64) then Divw rd rs1 rs2 else
-    if (opcode =? opcode_OP_32) && (funct3 =? funct3_DIVUW) && (funct7 =? funct7_DIVUW) && (xlen =? 64) then Divuw rd rs1 rs2 else
-    if (opcode =? opcode_OP_32) && (funct3 =? funct3_REMW) && (funct7 =? funct7_REMW) && (xlen =? 64) then Remw rd rs1 rs2 else
-    if (opcode =? opcode_OP_32) && (funct3 =? funct3_REMUW) && (funct7 =? funct7_REMUW) && (xlen =? 64) then Remuw rd rs1 rs2 else
-
-(* end decode *)
-    InvalidInstruction.
-
-
-Definition test_instruction: Z :=   Ox"0140006f".
-
-Definition test_result: Instruction := decode 32 test_instruction.
-
-Goal test_result = Jal 0 20.
-  reflexivity.
-Qed.
+(* Unbound variables:
+     Z Z.eqb Z.lor Z.shiftl andb bitSlice bool cons false list machineIntToShamt nil
+     orb signExtend true Coq.Init.Datatypes.app
+*)
