src/ExecuteI.v
@@ -1,219 +1,195 @@
-Require Import Coq.ZArith.BinInt.
-Require Import riscv.util.NameWithEq.
-Require Import riscv.RiscvBitWidths.
-Require Import riscv.util.Monads.
-Require Import riscv.Utility.
-Require Import riscv.Decode.
-Require Import riscv.Program.
+(* Default settings (from HsToCoq.Coq.Preamble) *)
 
-Local Open Scope Z.
+Generalizable All Variables.
+
+Unset Implicit Arguments.
+Set Maximal Implicit Insertion.
+Unset Strict Implicit.
+Unset Printing Implicit Defensive.
+
+Require Coq.Program.Tactics.
+Require Coq.Program.Wf.
+
+(* Preamble *)
+
+Require Import Utility.
 Local Open Scope alu_scope.
-Local Open Scope bool_scope.
 
-Section Riscv.
+(* Converted imports: *)
 
-  Context {Name: NameWithEq}. (* register name *)
-  Let Register := @name Name.
-  Existing Instance eq_name_dec.
+Require Decode.
+Require Import Monads.
+Require Import Program.
+Require Import Utility.
 
-  Context {B: RiscvBitWidths}.
+(* No type declarations to convert. *)
+(* Converted value declarations: *)
 
-  Context {M: Type -> Type}.
-  Context {MM: Monad M}.
-  Context {t: Set}.
-  Context {MW: MachineWidth t}.
-  Context {MP: MonadPlus M}.
-  Context {RVP: RiscvProgram M t}.
-  Context {RVS: RiscvState M t}.
-
-  Definition execute(i: Instruction): M unit :=
-    match i with
-    (* begin ast *)
-    | Lui rd imm20 =>
-        setRegister rd (fromImm imm20)
-    | Auipc rd oimm20 =>
-        pc <- getPC;
-        setRegister rd (fromImm oimm20 + pc)
-    | Jal rd jimm20 =>
-        pc <- getPC;
-        let newPC := pc + (fromImm jimm20) in
-        if (rem newPC four /= zero)
-          then raiseException zero zero
-          else (
-            setRegister rd (pc + four);;
-            setPC newPC)
-    | Jalr rd rs1 oimm12 =>
-        x <- getRegister rs1;
-        pc <- getPC;
-        let newPC := x + fromImm oimm12 in
-        if (rem newPC four /= zero)
-          then raiseException zero zero
-          else (
-            setRegister rd (pc + four);;
-            setPC newPC)
-    | Beq rs1 rs2 sbimm12 =>
-        x <- getRegister rs1;
-        y <- getRegister rs2;
-        pc <- getPC;
-        when (x == y) (
-          let newPC := (pc + fromImm sbimm12) in
-          if (rem newPC four /= zero)
-            then raiseException zero zero
-            else setPC newPC)
-    | Bne rs1 rs2 sbimm12 =>
-        x <- getRegister rs1;
-        y <- getRegister rs2;
-        pc <- getPC;
-        when (x /= y) (
-          let addr := (pc + fromImm sbimm12) in
-          if (rem addr four /= zero)
-            then raiseException zero zero
-            else setPC addr)
-    | Blt rs1 rs2 sbimm12 =>
-        x <- getRegister rs1;
-        y <- getRegister rs2;
-        pc <- getPC;
-        when (x < y) (
-          let addr := (pc + fromImm sbimm12) in
-          if (rem addr four /= zero)
-            then raiseException zero zero
-            else setPC addr)
-    | Bge rs1 rs2 sbimm12 =>
-        x <- getRegister rs1;
-        y <- getRegister rs2;
-        pc <- getPC;
-        when (x >= y) (
-          let addr := (pc + fromImm sbimm12) in
-          if (rem addr four /= zero)
-            then raiseException zero zero
-            else setPC addr)
-    | Bltu rs1 rs2 sbimm12 =>
-        x <- getRegister rs1;
-        y <- getRegister rs2;
-        pc <- getPC;
-        when ((ltu x y)) (
-          let addr := (pc + fromImm sbimm12) in
-          if (rem addr four /= zero)
-            then raiseException zero zero
-            else setPC addr)
-    | Bgeu rs1 rs2 sbimm12 =>
-        x <- getRegister rs1;
-        y <- getRegister rs2;
-        pc <- getPC;
-        when (negb (ltu x y)) (
-          let addr := (pc + fromImm sbimm12) in
-          if (rem addr four /= zero)
-            then raiseException zero zero
-            else setPC addr)
-    | Lb rd rs1 oimm12 =>
-        a <- getRegister rs1;
-        addr <- translate Load one (a + fromImm oimm12);
-        x <- loadByte addr;
-        setRegister rd (int8ToReg x)
-    | Lh rd rs1 oimm12 =>
-        a <- getRegister rs1;
-        addr <- translate Load two (a + fromImm oimm12);
-        x <- loadHalf addr;
-        setRegister rd (int16ToReg x)
-    | Lw rd rs1 oimm12 =>
-        a <- getRegister rs1;
-        addr <- translate Load four (a + fromImm oimm12);
-        x <- loadWord addr;
-        setRegister rd (int32ToReg x)
-    | Lbu rd rs1 oimm12 =>
-        a <- getRegister rs1;
-        addr <- translate Load one (a + fromImm oimm12);
-        x <- loadByte addr;
-        setRegister rd (uInt8ToReg x)
-    | Lhu rd rs1 oimm12 =>
-        a <- getRegister rs1;
-        addr <- translate Load two (a + fromImm oimm12);
-        x <- loadHalf addr;
-        setRegister rd (uInt16ToReg x)
-    | Sb rs1 rs2 simm12 =>
-        a <- getRegister rs1;
-        addr <- translate Store one (a + fromImm simm12);
-        x <- getRegister rs2;
-        storeByte addr (regToInt8 x)
-    | Sh rs1 rs2 simm12 =>
-        a <- getRegister rs1;
-        addr <- translate Store two (a + fromImm simm12);
-        x <- getRegister rs2;
-        storeHalf addr (regToInt16 x)
-    | Sw rs1 rs2 simm12 =>
-        a <- getRegister rs1;
-        addr <- translate Store four (a + fromImm simm12);
-        x <- getRegister rs2;
-        storeWord addr (regToInt32 x)
-    | Addi rd rs1 imm12 =>
-        x <- getRegister rs1;
-        setRegister rd (x + fromImm imm12)
-    | Slti rd rs1 imm12 =>
-        x <- getRegister rs1;
-        setRegister rd (if x < (fromImm imm12) then one else zero)
-    | Sltiu rd rs1 imm12 =>
-        x <- getRegister rs1;
-        setRegister rd (if (ltu x (fromImm imm12)) then one else zero)
-    | Xori rd rs1 imm12 =>
-        x <- getRegister rs1;
-        setRegister rd (xor x (fromImm imm12))
-    | Ori rd rs1 imm12 =>
-        x <- getRegister rs1;
-        setRegister rd (x <|> (fromImm imm12))
-    | Andi rd rs1 imm12 =>
-        x <- getRegister rs1;
-        setRegister rd (x <&> (fromImm imm12))
-    | Slli rd rs1 shamt6 =>
-        x <- getRegister rs1;
-        setRegister rd (sll x (regToShamt (fromImm shamt6 : t)))
-    | Srli rd rs1 shamt6 =>
-        x <- getRegister rs1;
-        setRegister rd (srl x (regToShamt (fromImm shamt6 : t)))
-    | Srai rd rs1 shamt6 =>
-        x <- getRegister rs1;
-        setRegister rd (sra x (regToShamt (fromImm shamt6 : t)))
-    | Add rd rs1 rs2 =>
-        x <- getRegister rs1;
-        y <- getRegister rs2;
-        setRegister rd (x + y)
-    | Sub rd rs1 rs2 =>
-        x <- getRegister rs1;
-        y <- getRegister rs2;
-        setRegister rd (x - y)
-    | Sll rd rs1 rs2 =>
-        x <- getRegister rs1;
-        y <- getRegister rs2;
-        setRegister rd (sll x (regToShamt y))
-    | Slt rd rs1 rs2 =>
-        x <- getRegister rs1;
-        y <- getRegister rs2;
-        setRegister rd (if x < y then one else zero)
-    | Sltu rd rs1 rs2 =>
-        x <- getRegister rs1;
-        y <- getRegister rs2;
-        setRegister rd (if (ltu x y) then one else zero)
-    | Xor rd rs1 rs2 =>
-        x <- getRegister rs1;
-        y <- getRegister rs2;
-        setRegister rd (xor x y)
-    | Or rd rs1 rs2 =>
-        x <- getRegister rs1;
-        y <- getRegister rs2;
-        setRegister rd (x <|> y)
-    | Srl rd rs1 rs2 =>
-        x <- getRegister rs1;
-        y <- getRegister rs2;
-        setRegister rd (srl x (regToShamt y))
-    | Sra rd rs1 rs2 =>
-        x <- getRegister rs1;
-        y <- getRegister rs2;
-        setRegister rd (sra x (regToShamt y))
-    | And rd rs1 rs2 =>
-        x <- getRegister rs1;
-        y <- getRegister rs2;
-        setRegister rd (x <&> y)
-    (* end ast *)
-    | _ => mzero
+Definition execute {p} {t} `{(RiscvState p t)}
+   : Decode.InstructionI -> p unit :=
+  fun arg_0__ =>
+    match arg_0__ with
+    | Decode.Lui rd imm20 => setRegister rd (fromImm imm20)
+    | Decode.Auipc rd oimm20 =>
+        Bind getPC (fun pc => setRegister rd (fromImm oimm20 + pc))
+    | Decode.Jal rd jimm20 =>
+        Bind getPC (fun pc =>
+                let newPC := pc + fromImm jimm20 in
+                if (rem newPC four /= zero) : bool
+                then raiseException zero zero
+                else (Bind (setRegister rd (pc + four)) (fun _ => setPC newPC)))
+    | Decode.Jalr rd rs1 oimm12 =>
+        Bind (getRegister rs1) (fun x =>
+                Bind getPC (fun pc =>
+                        let newPC := and (x + fromImm oimm12) (lnot one) in
+                        if (rem newPC four /= zero) : bool
+                        then raiseException zero zero
+                        else (Bind (setRegister rd (pc + four)) (fun _ => setPC newPC))))
+    | Decode.Beq rs1 rs2 sbimm12 =>
+        Bind (getRegister rs1) (fun x =>
+                Bind (getRegister rs2) (fun y =>
+                        Bind getPC (fun pc =>
+                                when (signed_eqb x y) (let newPC := (pc + fromImm sbimm12) in
+                                                       if (rem newPC four /= zero) : bool
+                                                       then raiseException zero zero
+                                                       else setPC newPC))))
+    | Decode.Bne rs1 rs2 sbimm12 =>
+        Bind (getRegister rs1) (fun x =>
+                Bind (getRegister rs2) (fun y =>
+                        Bind getPC (fun pc =>
+                                when (x /= y) (let addr := (pc + fromImm sbimm12) in
+                                               if (rem addr four /= zero) : bool
+                                               then raiseException zero zero
+                                               else setPC addr))))
+    | Decode.Blt rs1 rs2 sbimm12 =>
+        Bind (getRegister rs1) (fun x =>
+                Bind (getRegister rs2) (fun y =>
+                        Bind getPC (fun pc =>
+                                when (x < y) (let addr := (pc + fromImm sbimm12) in
+                                              if (rem addr four /= zero) : bool
+                                              then raiseException zero zero
+                                              else setPC addr))))
+    | Decode.Bge rs1 rs2 sbimm12 =>
+        Bind (getRegister rs1) (fun x =>
+                Bind (getRegister rs2) (fun y =>
+                        Bind getPC (fun pc =>
+                                when (x >= y) (let addr := (pc + fromImm sbimm12) in
+                                               if (rem addr four /= zero) : bool
+                                               then raiseException zero zero
+                                               else setPC addr))))
+    | Decode.Bltu rs1 rs2 sbimm12 =>
+        Bind (getRegister rs1) (fun x =>
+                Bind (getRegister rs2) (fun y =>
+                        Bind getPC (fun pc =>
+                                when ((ltu x y)) (let addr := (pc + fromImm sbimm12) in
+                                                  if (rem addr four /= zero) : bool
+                                                  then raiseException zero zero
+                                                  else setPC addr))))
+    | Decode.Bgeu rs1 rs2 sbimm12 =>
+        Bind (getRegister rs1) (fun x =>
+                Bind (getRegister rs2) (fun y =>
+                        Bind getPC (fun pc =>
+                                when (negb (ltu x y)) (let addr := (pc + fromImm sbimm12) in
+                                                       if (rem addr four /= zero) : bool
+                                                       then raiseException zero zero
+                                                       else setPC addr))))
+    | Decode.Lb rd rs1 oimm12 =>
+        Bind (getRegister rs1) (fun a =>
+                Bind (translate Load one (a + fromImm oimm12)) (fun addr =>
+                        Bind (loadByte addr) (fun x => setRegister rd (int8ToReg x))))
+    | Decode.Lh rd rs1 oimm12 =>
+        Bind (getRegister rs1) (fun a =>
+                Bind (translate Load two (a + fromImm oimm12)) (fun addr =>
+                        Bind (loadHalf addr) (fun x => setRegister rd (int16ToReg x))))
+    | Decode.Lw rd rs1 oimm12 =>
+        Bind (getRegister rs1) (fun a =>
+                Bind (translate Load four (a + fromImm oimm12)) (fun addr =>
+                        Bind (loadWord addr) (fun x => setRegister rd (int32ToReg x))))
+    | Decode.Lbu rd rs1 oimm12 =>
+        Bind (getRegister rs1) (fun a =>
+                Bind (translate Load one (a + fromImm oimm12)) (fun addr =>
+                        Bind (loadByte addr) (fun x => setRegister rd (uInt8ToReg x))))
+    | Decode.Lhu rd rs1 oimm12 =>
+        Bind (getRegister rs1) (fun a =>
+                Bind (translate Load two (a + fromImm oimm12)) (fun addr =>
+                        Bind (loadHalf addr) (fun x => setRegister rd (uInt16ToReg x))))
+    | Decode.Sb rs1 rs2 simm12 =>
+        Bind (getRegister rs1) (fun a =>
+                Bind (translate Store one (a + fromImm simm12)) (fun addr =>
+                        Bind (getRegister rs2) (fun x => storeByte addr (regToInt8 x))))
+    | Decode.Sh rs1 rs2 simm12 =>
+        Bind (getRegister rs1) (fun a =>
+                Bind (translate Store two (a + fromImm simm12)) (fun addr =>
+                        Bind (getRegister rs2) (fun x => storeHalf addr (regToInt16 x))))
+    | Decode.Sw rs1 rs2 simm12 =>
+        Bind (getRegister rs1) (fun a =>
+                Bind (translate Store four (a + fromImm simm12)) (fun addr =>
+                        Bind (getRegister rs2) (fun x => storeWord addr (regToInt32 x))))
+    | Decode.Addi rd rs1 imm12 =>
+        Bind (getRegister rs1) (fun x => setRegister rd (x + fromImm imm12))
+    | Decode.Slti rd rs1 imm12 =>
+        Bind (getRegister rs1) (fun x =>
+                setRegister rd (if x < fromImm imm12 : bool then one else zero))
+    | Decode.Sltiu rd rs1 imm12 =>
+        Bind (getRegister rs1) (fun x =>
+                setRegister rd (if (ltu x (fromImm imm12)) : bool then one else zero))
+    | Decode.Xori rd rs1 imm12 =>
+        Bind (getRegister rs1) (fun x => setRegister rd (xor x (fromImm imm12)))
+    | Decode.Ori rd rs1 imm12 =>
+        Bind (getRegister rs1) (fun x => setRegister rd (or x (fromImm imm12)))
+    | Decode.Andi rd rs1 imm12 =>
+        Bind (getRegister rs1) (fun x => setRegister rd (and x (fromImm imm12)))
+    | Decode.Slli rd rs1 shamt6 =>
+        Bind (getRegister rs1) (fun x => setRegister rd (sll x shamt6))
+    | Decode.Srli rd rs1 shamt6 =>
+        Bind (getRegister rs1) (fun x => setRegister rd (srl x shamt6))
+    | Decode.Srai rd rs1 shamt6 =>
+        Bind (getRegister rs1) (fun x => setRegister rd (sra x shamt6))
+    | Decode.Add rd rs1 rs2 =>
+        Bind (getRegister rs1) (fun x =>
+                Bind (getRegister rs2) (fun y => setRegister rd (x + y)))
+    | Decode.Sub rd rs1 rs2 =>
+        Bind (getRegister rs1) (fun x =>
+                Bind (getRegister rs2) (fun y => setRegister rd (x - y)))
+    | Decode.Sll rd rs1 rs2 =>
+        Bind (getRegister rs1) (fun x =>
+                Bind (getRegister rs2) (fun y => setRegister rd (sll x (regToShamt y))))
+    | Decode.Slt rd rs1 rs2 =>
+        Bind (getRegister rs1) (fun x =>
+                Bind (getRegister rs2) (fun y =>
+                        setRegister rd (if x < y : bool then one else zero)))
+    | Decode.Sltu rd rs1 rs2 =>
+        Bind (getRegister rs1) (fun x =>
+                Bind (getRegister rs2) (fun y =>
+                        setRegister rd (if (ltu x y) : bool then one else zero)))
+    | Decode.Xor rd rs1 rs2 =>
+        Bind (getRegister rs1) (fun x =>
+                Bind (getRegister rs2) (fun y => setRegister rd (xor x y)))
+    | Decode.Or rd rs1 rs2 =>
+        Bind (getRegister rs1) (fun x =>
+                Bind (getRegister rs2) (fun y => setRegister rd (or x y)))
+    | Decode.Srl rd rs1 rs2 =>
+        Bind (getRegister rs1) (fun x =>
+                Bind (getRegister rs2) (fun y => setRegister rd (srl x (regToShamt y))))
+    | Decode.Sra rd rs1 rs2 =>
+        Bind (getRegister rs1) (fun x =>
+                Bind (getRegister rs2) (fun y => setRegister rd (sra x (regToShamt y))))
+    | Decode.And rd rs1 rs2 =>
+        Bind (getRegister rs1) (fun x =>
+                Bind (getRegister rs2) (fun y => setRegister rd (and x y)))
+    | inst => Return tt
     end.
 
-End Riscv.
+(* Unbound variables:
+     Bind Load Return RiscvState Store and bool four fromImm getPC getRegister
+     int16ToReg int32ToReg int8ToReg lnot loadByte loadHalf loadWord ltu negb one
+     op_zgze__ op_zl__ op_zm__ op_zp__ op_zsze__ or raiseException regToInt16
+     regToInt32 regToInt8 regToShamt rem setPC setRegister signed_eqb sll sra srl
+     storeByte storeHalf storeWord translate tt two uInt16ToReg uInt8ToReg unit when
+     xor zero Decode.Add Decode.Addi Decode.And Decode.Andi Decode.Auipc Decode.Beq
+     Decode.Bge Decode.Bgeu Decode.Blt Decode.Bltu Decode.Bne Decode.InstructionI
+     Decode.Jal Decode.Jalr Decode.Lb Decode.Lbu Decode.Lh Decode.Lhu Decode.Lui
+     Decode.Lw Decode.Or Decode.Ori Decode.Sb Decode.Sh Decode.Sll Decode.Slli
+     Decode.Slt Decode.Slti Decode.Sltiu Decode.Sltu Decode.Sra Decode.Srai
+     Decode.Srl Decode.Srli Decode.Sub Decode.Sw Decode.Xor Decode.Xori
+*)
